adding two more verifying specs

pathSum.dfy
@@ -34,6 +34,38 @@ predicate isPath(paths: seq<TreeNode>, root: TreeNode) {
     }
 }
 
+function pathSum(paths: seq<TreeNode>): nat {
+    if |paths| == 0 then 0 else match paths[0] {
+        case Nil => 0
+        case Cons(val, left, right) => val + pathSum(paths[1..])
+    }
+}
+
+method hasPathSum(root: TreeNode, targetSum: int) returns (b: bool) 
+    ensures b ==> exists p: seq<TreeNode> :: isPath(p, root) && pathSum(p) == targetSum
+{
+    if root == Nil {
+        return false;
+    }
+
+    if(root.val - targetSum == 0 && root.left == Nil && root.right == Nil) {
+        assert isPath([root], root) && pathSum([root]) == targetSum;
+        return true;
+    }
+    var leftPath := hasPathSum(root.left, targetSum-root.val);
+    var rightPath := hasPathSum(root.right, targetSum-root.val);
+
+    if leftPath {
+        ghost var p: seq<TreeNode> :| isPath(p, root.left) && pathSum(p) == targetSum-root.val;
+        assert isPath([root]+p, root) && pathSum([root]+p) == targetSum;
+    }
+    if rightPath {
+        ghost var p: seq<TreeNode> :| isPath(p, root.right) && pathSum(p) == targetSum-root.val;
+        assert isPath([root]+p, root) && pathSum([root]+p) == targetSum;
+    }
+    return leftPath || rightPath;
+}
+
 method Test() {
     var c := Cons(3, Nil, Nil);
     var b := Cons(2, c, Nil);
