MinDepth.dfy
@@ -1,0 +1,124 @@
+
+datatype TreeNode = Nil | Cons(val: nat, left: TreeNode, right: TreeNode)
+
+predicate isPath(paths: seq<TreeNode>, root: TreeNode) {
+    if |paths| == 0 then false else match paths[0] {
+        case Nil => false
+        case Cons(val, left, right) => if |paths| == 1 then root == paths[0] else root == paths[0] && (isPath(paths[1..], left) || isPath(paths[1..], right))
+    }
+}
+
+function TreeSet(root: TreeNode): set<TreeNode> {
+    match root {
+        case Nil => {Nil}
+        case Cons(val, left, right) => TreeSet(left)+{root}+TreeSet(right)
+    }
+}
+
+function ChildSet(root: TreeNode): set<TreeNode> {
+    match root {
+        case Nil => {Nil}
+        case Cons(val, left, right) => {left}+ChildSet(left)+{right}+ChildSet(right)
+    }
+}
+
+function method max(a:int,b: int): int {
+    if a > b then a else b
+}
+
+function method min(a:int,b: int): int {
+    if a > b then b else a
+}
+
+function method boundedMin(a: int, b: int): int {
+    if a == 0 then b else if b == 0 then a else min(a,b)
+}
+
+function TreeHeight(root: TreeNode): nat {
+    match root {
+        case Nil => 0
+        case Cons(val, Nil, Nil) => 1
+        case Cons(val, left, right) => 1 + max(TreeHeight(left), TreeHeight(right))
+    }
+}
+
+method minDepth(root: TreeNode) returns (depth: nat) 
+    requires forall node :: node in TreeSet(root) ==> node !in ChildSet(node)
+    ensures depth > 0 ==> exists p: seq<TreeNode> :: isPath(p, root) && |p| == depth
+    // ensures depth > 0 ==> forall ps: seq<TreeNode> :: isPath(ps, root) ==> depth <= |ps|
+{
+    if root == Nil {
+        return 0;
+    }
+
+    if root.left == Nil && root.right == Nil {
+        assert isPath([root], root) && |[root]| == 1;
+        return 1;
+    }
+    var leftDepth := minDepth(root.left);
+    var rightDepth := minDepth(root.right);
+    if leftDepth > 0 {
+        // ghost var q: seq<TreeNode> :| isPath(q, root.left) && |q| == leftDepth && forall ps: seq<TreeNode> :: isPath(ps, root.left) ==> leftDepth <= |ps|;
+        ghost var q: seq<TreeNode> :| isPath(q, root.left) && |q| == leftDepth;
+        assert isPath([root]+q, root) && |[root]+q| == 1 + leftDepth;
+    }
+    if rightDepth > 0 {
+        ghost var p: seq<TreeNode> :| isPath(p, root.right) && |p| == rightDepth;
+        assert isPath([root]+p, root) && |[root]+p| == 1 + rightDepth;
+    }
+    // if leftDepth > 0 && rightDepth > 0 {
+    //     ghost var q: seq<TreeNode> :| isPath(q, root.left) && |q| == leftDepth && forall ps: seq<TreeNode> :: isPath(ps, root.left) ==> leftDepth <= |ps|;
+    //     ghost var p: seq<TreeNode> :| isPath(p, root.right) && |p| == rightDepth && forall ps: seq<TreeNode> :: isPath(ps, root.right) ==> rightDepth <= |ps|;
+    //     ghost var ps := set px: seq<TreeNode> | isPath(px, root) ; 
+    //     if leftDepth > rightDepth {
+    //         // assert forall ps: seq<TreeNode> :: isPath([root]+q, root) ==> 1+boundedMin(leftDepth, rightDepth) <= |p|;
+
+    //     }else if rightDepth > leftDepth {
+
+    //     }else{
+
+    //     }
+    // }
+    return 1 + boundedMin(leftDepth, rightDepth);
+}
+
+// lemma MinDepthMinimal(root: TreeNode, path: seq<TreeNode>, depth: nat) 
+//     requires isPath(path, root)
+//     requires depth == |path| && depth > 0
+//     ensures forall ps: seq<TreeNode> :: isPath(ps, root) && ps != path ==> depth <= |ps|
+// {
+//     var what := minDepth(root);
+// }
+
+/**
+    showing minimum
+    if both |ps| == |p| == 1 then true
+    assume that another path (ps, root) exists and it is not equal to path(p,root) and it is less than |p|;
+    assume forall isPath(ps, root) ==> |p| <= |ps|
+
+    then either p && ps include root and root.left in which case mindDepth root.left == root.right
+    then either p && ps include root and root.right
+    then either p includes root.right and ps includes root.left
+    |ps| < |p| ==> |ps|+1 < |p| + 1
+    rightDepth == |ps|
+    leftDepth == |p|
+    
+    then either p includes root.left and ps includes root.right
+    |ps| < |p| ==> |ps|+1 < |p| + 1
+    rightDepth == |p|
+    leftDepth == |ps|
+
+ (!forall ps: seq<TreeNode> :: isPath(ps, root) ==> depth <= |ps|) 
+exists ps(ps root) && depth > |ps|
+
+
+ */
+
+method Test() {
+    var t := Nil;
+    assert TreeHeight(t) == 0;
+    var t1 := Cons(3,Nil, Nil);
+    assert TreeHeight(t1) == 1;
+    var t2 := Cons(3,Nil, Cons(4, Nil, Nil));
+    assert TreeHeight(t2) == 2;
+}
